src/Assembly/MultiBoundedWord.v
@@ -1,0 +1,116 @@
+
+Require Import Bedrock.Word Bedrock.Nomega.
+Require Import NArith PArith Ndigits Compare_dec Arith.
+Require Import ProofIrrelevance Ring.
+Require Import BoundedWord.
+
+Section MultiBoundedWord.
+  Import BoundedWord.
+
+  (* Parameters of boundedness calculations *)
+  Delimit Scope Bounded_scope with bounded.
+  Open Scope Bounded_scope.
+
+  Context {n: nat}.
+
+  Notation "A <= B" := (wordLeN A B) (at level 70) : Bounded_scope.
+  Notation "$" := (natToWord n) : Bounded_scope.
+
+  (* Hypothesis-based word-bound tactic *)
+  Ltac multi_apply0 A L := pose proof (L A).
+
+  Ltac multi_apply1 A L :=
+    match goal with
+    | [ H: A <= ?b |- _] => pose proof (L A b H)
+    end.
+
+  Ltac multi_apply2 A B L :=
+    match goal with
+    | [ H1: A <= ?b1, H2: B <= ?b2 |- _] => pose proof (L A B b1 b2 H1 H2)
+    end.
+
+  Ltac multi_recurse T :=
+    match goal with
+    | [ H: T <= _ |- _] => idtac
+    | _ =>
+      match T with
+      | ?W1 ^+ ?W2 =>
+        multi_recurse W1; multi_recurse W2;
+        multi_apply2 W1 W2 (@wplus_bound n)
+
+      | ?W1 ^* ?W2 =>
+        multi_recurse W1; multi_recurse W2;
+        multi_apply2 W1 W2 (@wmult_bound n)
+
+      | mask ?m ?w <= (N.min _ (Npow2 _ - 1)) =>
+        multi_recurse w;
+        multi_apply1 w (@mask_update_bound n)
+
+      | shiftr ?w ?bits <= N.shiftr ?b (N.of_nat _) =>
+        multi_recurse w;
+        match goal with
+        | [ H: w <= ?b |- _] =>
+          pose proof (@shiftr_bound n w b bits H)
+        end
+
+      | NToWord n ?k => pose proof (@constant_bound_N n k)
+
+      | natToWord n ?k <= _ => pose proof (@constant_bound_nat n k)
+
+      | ($ ?k) => pose proof (@constant_bound_nat n k)
+
+      | _ => pose proof (@word_size_bound n T)
+      end
+    end.
+
+  Lemma unwrap_let: forall (y: word n) (f: word n -> word n) (b: N),
+      (let x := y in f x) <= b <-> let x := y in (f x <= b).
+  Proof. intuition. Qed.
+
+  Ltac multi_bound :=
+    match goal with
+    | [|- let A := ?B in _] =>
+      multi_recurse B; intro; unfold A; multi_bound
+    | [|- (let A := _ in _) <= _] =>
+      apply unwrap_let; multi_bound
+    | [|- ?W <= _ ] => multi_recurse W
+    end.
+
+  (* Examples *)
+  Lemma example1 : forall (w1 w2 w3 w4 : word n) b1 b2 b3 b4,
+    w1 <= b1
+    -> w2 <= b2
+    -> w3 <= b3
+    -> w4 <= b4
+    -> { b | let w5 := w2 ^* w3 in w1 ^+ w5 ^* w4 <= b }.    
+  Proof.
+    eexists.
+    multi_bound.
+    eassumption.
+  Defined.
+
+  Lemma example2 : forall (w1 w2 w3 w4 : word n) b1 b2 b3 b4,
+    w1 <= b1
+    -> w2 <= b2
+    -> w3 <= b3
+    -> w4 <= b4
+    -> { b | (let w5 := (w2 ^* $7 ^* w3) in w1 ^+ w5 ^* w4 ^+ $8 ^+ w2) <= b }.
+  Proof.
+    eexists.
+    multi_bound.
+    eassumption.
+  Defined.
+
+  Lemma example3 : forall (w1 w2 w3 w4 : word n),
+    w1 <= Npow2 3
+    -> w2 <= Npow2 4
+    -> w3 <= Npow2 8
+    -> w4 <= Npow2 16
+    -> { b | w1 ^+ (w2 ^* $7 ^* w3) ^* w4 ^+ $8 ^+ w2 <= b }.
+  Proof.
+    eexists.
+    multi_bound.
+    eassumption.
+  Defined.
+
+End MultiBoundedWord.
